test-suite/loop-checking/theories/LoopCheckingPlugin.v
@@ -21,7 +21,7 @@ Local Open Scope monad_scope.
 Global Instance TemplateMonad_Monad@{t u} : Monad@{t u} TM@{t} :=
   {| ret := @tmReturn ; bind := @tmBind |}.
 
-Definition check_universes  : TM unit :=
+Definition check_universes : TM unit :=
   tmQuoteUniverses >>= fun ctx =>
   let clauses := time "building clauses" enforce_level_constraints (snd ctx) in
   tmMsg (string_of_nat (LevelSet.cardinal (fst ctx)) ++ " universes and " ++ string_of_nat (ConstraintSet.cardinal (snd ctx)) ++ " constraints") ;;
